Semantics/IRStepThms.thy
@@ -103,9 +103,9 @@ proof (induction rule: "step.induct")
     by (metis is_IntegerDivRemNode.simps SequentialNode.hyps(1) is_sequential_node.simps(45,46)
         is_SignedDivNode_def is_SignedRemNode_def)
   from notif notend notnew notload notstore notdivrem
-  show ?case 
-    by (smt (verit) SequentialNode step.cases is_sequential_node.simps(17,19,28,36,45,46,47)
-        Pair_inject IRNode.discI(32))
+  show ?case
+    by (smt (verit) SequentialNode step.cases is_sequential_node.simps(11,17,19,45,46) Pair_inject
+        IRNode.discI(33) IRNode.disc(1178,2466))
 next
   case (FixedGuardNode nid cond before "next" condE m p val h)
   have notseq: "\<not>(is_sequential_node (kind g nid))"
@@ -114,8 +114,8 @@ next
     by (simp add: FixedGuardNode.hyps(1))
   from notseq notend 
   show ?case
-    by (smt (verit) FixedGuardNode.hyps(1,5) IRNode.distinct(993,1013,1035,1053,1055,1059)
-        step.simps Pair_inject IRNode.inject(10))
+    by (smt (verit) FixedGuardNode.hyps(1,5) IRNode.distinct(431,993,1013,1035,1053,1055,1059)
+        step.cases Pair_inject IRNode.inject(10))
 next
   case (IfNode nid cond tb fb m val "next" h)
   then have notseq: "\<not>(is_sequential_node (kind g nid))"
@@ -124,9 +124,34 @@ next
     by (simp add: IfNode.hyps(1))
   have notdivrem: "\<not>(is_IntegerDivRemNode (kind g nid))" 
     by (simp add: IfNode.hyps(1))
-  from notseq notend notdivrem show ?case
-    by (smt (verit) IRNode.inject(11,12) Pair_inject step.simps IfNode repDet evalDet
-        IRNode.distinct(993,1183,1205,1223,1225,1229))
+  from notseq notend notdivrem
+  show ?case
+    by (smt (verit) IRNode.inject(12) Pair_inject repDet evalDet IfNode.hyps(1,2,3,4) step.cases
+        IRNode.distinct(435,993,1183,1205,1223,1225,1229))
+next
+  case (BytecodeExceptionNode nid args st n' ex h' ref h m' m)
+  have notseq: "\<not>(is_sequential_node (kind g nid))"
+    by (simp add: BytecodeExceptionNode.hyps(1))
+  have notif: "\<not>(is_IfNode (kind g nid))"
+    by (simp add: BytecodeExceptionNode.hyps(1))
+  have notref: "\<not>(is_RefNode (kind g nid))"
+    by (metis notseq is_RefNode_def is_sequential_node.simps(7))
+  have notnew: "\<not>(is_NewInstanceNode (kind g nid))"
+    by (simp add: BytecodeExceptionNode.hyps(1))
+  have notload: "\<not>(is_LoadFieldNode (kind g nid))"
+    by (simp add: BytecodeExceptionNode.hyps(1))
+  have notstore: "\<not>(is_StoreFieldNode (kind g nid))"
+    by (simp add: BytecodeExceptionNode.hyps(1))
+  have notdivrem: "\<not>(is_IntegerDivRemNode (kind g nid))"
+    by (simp add: BytecodeExceptionNode.hyps(1))
+  have notfixedguard: "\<not>(is_FixedGuardNode (kind g nid))"
+    by (simp add: BytecodeExceptionNode.hyps(1))
+  have notend: "\<not>(is_AbstractEndNode (kind g nid))"
+    by (simp add: BytecodeExceptionNode.hyps(1))
+  from notseq notif notref notnew notload notstore notdivrem notfixedguard notend
+  show ?case
+    by (smt (verit) BytecodeExceptionNode.hyps(1,2,3,4) IRNode.disc(506,1178,2466) IRNode.inject(5)
+        IRNode.discI(12,33) IRNode.distinct(495,497) Pair_inject step.cases repDet)
 next
   case (EndNodes nid merge i phis inputs m vs m' h)
   have notseq: "\<not>(is_sequential_node (kind g nid))"
@@ -151,11 +176,15 @@ next
   have notfixedguard: "\<not>(is_FixedGuardNode (kind g nid))"
     by (metis IRNode.distinct_disc(1019) is_EndNode.simps(11) is_FixedGuardNode_def EndNodes.hyps(1)
         is_AbstractEndNode.simps)
-  from notseq notif notref notnew notload notstore notdivrem notfixedguard
+  have notbytecodeexception: "\<not>(is_BytecodeExceptionNode (kind g nid))"
+    by (metis IRNode.distinct_disc(461) is_BytecodeExceptionNode_def is_AbstractEndNode.simps
+        is_EndNode.simps(6) EndNodes.hyps(1))
+  from notseq notif notref notnew notload notstore notdivrem notfixedguard notbytecodeexception
   show ?case 
     by (smt (verit) IRNode.disc(497,506) repAllDet evalAllDet is_IfNode_def EndNodes step.cases
         is_RefNode_def Pair_inject is_LoadFieldNode_def is_NewInstanceNode_def is_StoreFieldNode_def
-        is_SignedDivNode_def is_SignedRemNode_def is_IntegerDivRemNode.elims(3))
+        is_SignedDivNode_def is_SignedRemNode_def is_IntegerDivRemNode.elims(3)
+        is_BytecodeExceptionNode_def)
 next
   case (NewInstanceNode nid f obj nxt h' ref h m' m)
   then have notseq: "\<not>(is_sequential_node (kind g nid))"
@@ -175,7 +204,7 @@ next
   from notseq notend notif notref notload notstore notdivrem
   show ?case 
     by (smt (verit) NewInstanceNode step.cases IRNode.disc(1102,1013,1178,2367,2417,2419,2466)
-        IRNode.discI(12) Pair_inject IRNode.distinct(1035,2525,2527) IRNode.inject(32,33))
+        IRNode.discI(12) Pair_inject IRNode.distinct(477,1035,2525,2527) IRNode.inject(32,33))
 next
   case (LoadFieldNode nid f obj nxt m ref h v m')
   then have notseq: "\<not>(is_sequential_node (kind g nid))"
@@ -187,7 +216,7 @@ next
   from notseq notend notdivrem
   show ?case 
     by (smt (verit) LoadFieldNode step.cases repDet evalDet IRNode.inject(21,22) option.distinct(1)
-        IRNode.distinct(991,1013,1157,1183,1827,1845,1847,1851,1935,1953,1955,1959) Pair_inject
+        IRNode.distinct(455,991,1013,1157,1183,1827,1845,1847,1851,1935,1953,1955,1959) Pair_inject
         Value.inject(2) option.inject)
 next
   case (StaticLoadFieldNode nid f nxt h v m' m)
@@ -198,8 +227,8 @@ next
   have notdivrem: "\<not>(is_IntegerDivRemNode (kind g nid))"
     by (simp add: StaticLoadFieldNode.hyps(1))
   from notseq notend notdivrem
-  show ?case  
-    by (smt (verit) IRNode.distinct(991,1013,1157,1183,1827,1845,1847,1851,1935,1953,1955,1959)
+  show ?case
+    by (smt (verit) IRNode.distinct(455,991,1013,1157,1183,1827,1845,1847,1851,1935,1953,1955,1959)
         IRNode.inject(21,22) StaticLoadFieldNode step.cases Pair_inject option.distinct(1))
 next
   case (StoreFieldNode nid f newval uu obj nxt m val ref h' h m')
@@ -211,7 +240,7 @@ next
     by (simp add: StoreFieldNode.hyps(1))
   from notseq notend notdivrem
   show ?case 
-    by (smt (verit) IRNode.distinct(1037,1059,1203,1229,1851,1959,2423,2531,2711,2733,2819,2841)
+    by (smt (verit) IRNode.distinct(501,1037,1059,1203,1229,1851,1959,2423,2531,2711,2733,2819,2841)
         IRNode.inject(44,45) StoreFieldNode step.cases repDet evalDet option.distinct(1) Pair_inject
         Value.inject(2) option.inject)
 next
@@ -224,7 +253,7 @@ next
     by (simp add: StaticStoreFieldNode.hyps(1))
   from notseq notend notdivrem
   show ?case  
-    by (smt (verit) IRNode.distinct(1037,1059,1203,1229,1851,1959,2423,2531,2711,2733,2819,2841)
+    by (smt (verit) IRNode.distinct(501,1037,1059,1203,1229,1851,1959,2423,2531,2711,2733,2819,2841)
         IRNode.inject(44,45) StoreFieldNode repDet evalDet StaticStoreFieldNode.hyps(1,2,3,4,5)
         Pair_inject option.distinct(1) step.cases)
 next
@@ -234,8 +263,8 @@ next
   have notend: "\<not>(is_AbstractEndNode (kind g nid))"
     by (simp add: SignedDivNode.hyps(1))
   from notseq notend
-  show ?case  
-    by (smt (verit) IRNode.distinct(1031,1053,1197,1223,1845,1953,2417,2525,2707,2711,2815,2819)
+  show ?case
+    by (smt (verit) IRNode.distinct(495,1031,1053,1197,1223,1845,1953,2417,2525,2707,2711,2815,2819)
         IRNode.inject(42) SignedDivNode IRNode.inject(41) step.cases repDet evalDet Pair_inject)
 next
   case (SignedRemNode nid x y zero sb nxt m v1 v2 v m' h)
@@ -245,7 +274,7 @@ next
     by (simp add: SignedRemNode.hyps(1))
   from notseq notend
   show ?case 
-    by (smt (verit) IRNode.distinct(1033,1055,1199,1225,1847,1955,2419,2527,2707,2733,2815,2841)
+    by (smt (verit) IRNode.distinct(497,1033,1055,1199,1225,1847,1955,2419,2527,2707,2733,2815,2841)
         IRNode.inject(43) SignedRemNode IRNode.inject(42) step.cases repDet evalDet Pair_inject)
 qed
 
@@ -275,7 +304,7 @@ lemma step_in_ids:
   assumes "g, p \<turnstile> (nid, m, h) \<rightarrow> (nid', m', h')"
   shows "nid \<in> ids g"
   using assms apply (induct "(nid, m, h)" "(nid', m', h')" rule: step.induct) apply fastforce
-  by (metis IRNode.distinct(1075,1245,1975,2547,2835,2857,2895) IRNode.disc(1374,2895) ids_some
+  by (metis IRNode.distinct(517,1075,1245,1975,2547,2835,2857,2895) IRNode.disc(1374) ids_some
       is_EndNode.simps(54) is_AbstractEndNode.simps)+
 
 end
